\documentclass[journal,11pt]{IEEEtran}
\usepackage{setspace}
\usepackage{gensymb}
\singlespacing
\usepackage[cmex10]{amsmath}
\usepackage{amsthm}
\usepackage{mathrsfs}
\usepackage{txfonts}
\usepackage{stfloats}
\usepackage{bm}
\usepackage{cite}
\usepackage{cases}
\usepackage{subfig}
\usepackage{longtable}
\usepackage{multirow}
\usepackage{enumitem}
\usepackage{mathtools}
\usepackage{tikz}
\usepackage{circuitikz}
\usepackage{verbatim}
\usepackage[breaklinks=true]{hyperref}
\usepackage{tkz-euclide} % loads  TikZ and tkz-base
\usepackage{listings}
\usepackage{color}    
\usepackage{array}    
\usepackage{longtable}
\usepackage{calc}     
\usepackage{multirow} 
\usepackage{hhline}   
\usepackage{ifthen}   
\usepackage{lscape}     
\usepackage{chngcntr}
\usepackage{float}
\usepackage{gvv}

\begin{document}

\vspace{3cm}
\author{Ajay Krishnan K\\EE22BTECH11003}

\title{Gate ST-37.2023}
\maketitle

\textbf{Question}
Let $X$ be a random variable with probability density function
\begin{align}\
    % align the cases
    f(x) = \begin{cases}
        \frac{1}{x^2} & if x \geq 1\\
        0  & otherwise.
        \end{cases}
\end{align}
If $Y = \log_e X$, then $\pr{Y<1 | Y<2 }$ equals

\solution
Given, the probability density function of $X$ is
\begin{align}
    f(x) = \begin{cases}
        \frac{1}{x^2} & if x \geq 1\\
        0  & otherwise.
        \end{cases}
\end{align}
Also, $Y = \log_e X$.\\
Consider the cumulative distribution function(CDF) of $Y$,
\begin{align}
    F_Y(y) &= \pr{Y \leq y}\\
    &= \pr{\log_e X \leq y}\\
    &= \pr{X \leq e^y}\\
    &= \int_{1}^{e^y} \frac{1}{x^2} dx\\
    &= 1 - \frac{1}{e^y}
\end{align}
Now, we need to find $\pr{Y<1 | Y<2 }$.
For that, we need to find $F_Y(1)$ and $F_Y(2)$.\\
Using the equation for CDF,
\begin{align}
    F_Y(1) &= 1 - \frac{1}{e}
\end{align}
and
\begin{align}
    F_Y(2) &= 1 - \frac{1}{e^2}
\end{align}

Now, we can find $\pr{Y<1 | Y<2 }$ as follows,
\begin{align}
    \pr{Y<1 | Y<2 } &= \frac{\pr{Y<1 , Y<2}}{\pr{Y<2}}\\
    &= \frac{\pr{Y<1}}{\pr{Y<2}}\\
    &= \frac{F_Y(1)}{F_Y(2)}\\
    &= \frac{1 - \frac{1}{e}}{1 - \frac{1}{e^2}}\\
    &= \frac{e(e-1)}{e^2-1}\\
    &= \frac{e}{e+1}
\end{align}

\end{document}
